README.md
@@ -44,3 +44,4 @@ Hello Corny
  * String handling
  * `println "foo" >> println "bar"` and a *proof* that I got `foo\nbar\n` on my stdout
  * `now >>= \time -> println $ "the time is now " ++ time`
+ * Read a number from stdin, increment the number and output it
